Change system rules (#157)
* Refactor system rule

* Enhance System for Soundness

* Update SubtypingCases.v

* Clear System.v Up

theories/Core/Syntactic/System/Definitions.v
@@ -80,8 +80,18 @@ with wf_exp : ctx -> typ -> exp -> Prop :=
   `( {{ Γ ⊢s σ : Δ }} ->
      {{ Δ ⊢ M : A }} ->
      {{ Γ ⊢ M[σ] : A[σ] }} )
-| wf_subtyp :
+| wf_exp_subtyp :
   `( {{ Γ ⊢ M : A }} ->
+     (** We have this extra argument for soundness.
+         Note that we need to keep it asymmetric:
+         only [A'] is checked. If we check A as well,
+         we cannot even construct something like
+         [{{ Γ ⊢ Type@0[Wk] : Type@1 }}] with the current
+         rules. Under the symmetric rule, the example requires
+         [{{ Γ ⊢ Type@1[Wk] : Type@2 }}] to apply [wf_exp_sub],
+         which requires [{{ Γ ⊢ Type@2[Wk] : Type@3 }}], and so on.
+      *)
+     {{ Γ ⊢ A' : Type@i }} ->
      {{ Γ ⊢ A ⊆ A' }} ->
      {{ Γ ⊢ M : A' }} )
 where "Γ ⊢ M : A" := (wf_exp Γ A M) (in custom judg) : type_scope
@@ -104,6 +114,11 @@ with wf_sub : ctx -> ctx -> sub -> Prop :=
      {{ Γ ⊢s (σ ,, M) : Δ , A }} )
 | wf_sub_subtyp :
   `( {{ Γ ⊢s σ : Δ }} ->
+     (** As in [wf_exp_subtyp], this extra argument is
+         for soundness. We don't need to keep it asymmetric,
+         but do so to match with [wf_exp_subtyp].
+      *)
+     {{ ⊢ Δ' }} ->
      {{ ⊢ Δ ⊆ Δ' }} ->
      {{ Γ ⊢s σ : Δ' }} )
 where "Γ ⊢s σ : Δ" := (wf_sub Γ Δ σ) (in custom judg) : type_scope
@@ -225,11 +240,12 @@ with wf_exp_eq : ctx -> typ -> exp -> exp -> Prop :=
      {{ Γ' ⊢s σ : Γ'' }} ->
      {{ Γ'' ⊢ M : A }} ->
      {{ Γ ⊢ M[σ ∘ τ] ≈ M[σ][τ] : A[σ ∘ τ] }} )
-| wf_exp_eq_cumu :
-  `( {{ Γ ⊢ A ≈ A' : Type@i }} ->
-     {{ Γ ⊢ A ≈ A' : Type@(S i) }} )
 | wf_exp_eq_subtyp :
   `( {{ Γ ⊢ M ≈ M' : A }} ->
+     {{ Γ ⊢ A' : Type@i }} ->
+     (** This extra argument is here to be consistent with
+         [wf_exp_subtyp].
+      *)
      {{ Γ ⊢ A ⊆ A' }} ->
      {{ Γ ⊢ M ≈ M' : A' }} )
 | wf_exp_eq_sym :
@@ -291,13 +307,27 @@ with wf_sub_eq : ctx -> ctx -> sub -> sub -> Prop :=
      {{ Γ ⊢s σ ≈ σ'' : Δ }} )
 | wf_sub_eq_subtyp :
   `( {{ Γ ⊢s σ ≈ σ' : Δ }} ->
+     (** This extra argument is here to be consistent with
+         [wf_sub_subtyp].
+      *)
+     {{ ⊢ Δ' }} ->
      {{ ⊢ Δ ⊆ Δ' }} ->
      {{ Γ ⊢s σ ≈ σ' : Δ' }} )
 where "Γ ⊢s S1 ≈ S2 : Δ" := (wf_sub_eq Γ Δ S1 S2) (in custom judg) : type_scope
 
-with wf_subtyping : ctx -> typ -> typ -> Prop :=
+with wf_subtyp : ctx -> typ -> typ -> Prop :=
 | wf_subtyp_refl :
-  `( {{ Γ ⊢ M ≈ M' : Type@i }} ->
+  (** We need this extra argument in order to prove the lemmas
+      in CtxSub.v independently. We can prove those and
+      presupposition lemmas mutually dependently, but that would
+      be more messy.
+
+      The main point of this assumption gives presupposition for
+      RHS directly so that we can remove the extra arguments in
+      type checking rules immediately.
+   *)
+  `( {{ Γ ⊢ M' : Type@i }} ->
+     {{ Γ ⊢ M ≈ M' : Type@i }} ->
      {{ Γ ⊢ M ⊆ M' }} )
 | wf_subtyp_trans :
   `( {{ Γ ⊢ M ⊆ M' }} ->
@@ -315,7 +345,7 @@ with wf_subtyping : ctx -> typ -> typ -> Prop :=
      {{ Γ , A' ⊢ B' : Type@i }} ->
      {{ Γ , A' ⊢ B ⊆ B' }} ->
      {{ Γ ⊢ Π A B ⊆ Π A' B' }} )
-where "Γ ⊢ A ⊆ A'" := (wf_subtyping Γ A A') (in custom judg) : type_scope.
+where "Γ ⊢ A ⊆ A'" := (wf_subtyp Γ A A') (in custom judg) : type_scope.
 
 Scheme wf_ctx_mut_ind := Induction for wf_ctx Sort Prop
 with wf_ctx_sub_mut_ind := Induction for wf_ctx_sub Sort Prop
@@ -323,7 +353,7 @@ with wf_exp_mut_ind := Induction for wf_exp Sort Prop
 with wf_exp_eq_mut_ind := Induction for wf_exp_eq Sort Prop
 with wf_sub_mut_ind := Induction for wf_sub Sort Prop
 with wf_sub_eq_mut_ind := Induction for wf_sub_eq Sort Prop
-with wf_subtyping_mut_ind := Induction for wf_subtyping Sort Prop.
+with wf_subtyp_mut_ind := Induction for wf_subtyp Sort Prop.
 Combined Scheme syntactic_wf_mut_ind from
   wf_ctx_mut_ind,
   wf_ctx_sub_mut_ind,
@@ -331,7 +361,7 @@ Combined Scheme syntactic_wf_mut_ind from
   wf_exp_eq_mut_ind,
   wf_sub_mut_ind,
   wf_sub_eq_mut_ind,
-  wf_subtyping_mut_ind.
+  wf_subtyp_mut_ind.
 
 Scheme wf_ctx_mut_ind' := Induction for wf_ctx Sort Prop
 with wf_exp_mut_ind' := Induction for wf_exp Sort Prop
@@ -346,6 +376,8 @@ Inductive wf_ctx_eq : ctx -> ctx -> Prop :=
 | wf_ctx_eq_extend :
   `( {{ ⊢ Γ ≈ Δ }} ->
      {{ Γ ⊢ A : Type@i }} ->
+     {{ Γ ⊢ A' : Type@i }} ->
+     {{ Δ ⊢ A : Type@i }} ->
      {{ Δ ⊢ A' : Type@i }} ->
      {{ Γ ⊢ A ≈ A' : Type@i }} ->
      {{ Δ ⊢ A ≈ A' : Type@i }} ->
@@ -353,10 +385,10 @@ Inductive wf_ctx_eq : ctx -> ctx -> Prop :=
 where "⊢ Γ ≈ Γ'" := (wf_ctx_eq Γ Γ') (in custom judg) : type_scope.
 
 #[export]
-Hint Constructors wf_ctx wf_ctx_eq wf_ctx_sub wf_exp wf_sub wf_exp_eq wf_sub_eq wf_subtyping ctx_lookup : mcltt.
+Hint Constructors wf_ctx wf_ctx_eq wf_ctx_sub wf_exp wf_sub wf_exp_eq wf_sub_eq wf_subtyp ctx_lookup : mcltt.
 
 #[export]
-Instance wf_exp_PER Γ A : PER (wf_exp_eq Γ A).
+Instance wf_exp_eq_PER Γ A : PER (wf_exp_eq Γ A).
 Proof.
   split.
   - eauto using wf_exp_eq_sym.
@@ -364,7 +396,7 @@ Proof.
 Qed.
 
 #[export]
-Instance wf_sub_PER Γ Δ : PER (wf_sub_eq Γ Δ).
+Instance wf_sub_eq_PER Γ Δ : PER (wf_sub_eq Γ Δ).
 Proof.
   split.
   - eauto using wf_sub_eq_sym.
@@ -372,34 +404,133 @@ Proof.
 Qed.
 
 #[export]
-  Instance wf_subtyping_trans Γ : Transitive (wf_subtyping Γ).
+Instance wf_ctx_eq_Symmetric : Symmetric wf_ctx_eq.
+Proof.
+  induction 1; mauto.
+Qed.
+
+#[export]
+Instance wf_subtyp_Transitive Γ : Transitive (wf_subtyp Γ).
 Proof.
   hnf; mauto.
 Qed.
 
+(** Immediate & Independent Presuppositions *)
 
-Add Parametric Morphism i Γ : (wf_exp Γ)
-    with signature wf_exp_eq Γ {{{ Type@i }}} ==> eq ==> iff as wf_exp_morph.
-Proof.
-  intros; split; mauto.
+Lemma presup_ctx_sub : forall {Γ Δ}, {{ ⊢ Γ ⊆ Δ }} -> {{ ⊢ Γ }} /\ {{ ⊢ Δ }}.
+Proof with mautosolve.
+  induction 1; destruct_pairs...
 Qed.
 
-Add Parametric Morphism i Γ : (wf_exp_eq Γ)
-    with signature wf_exp_eq Γ {{{ Type@i }}} ==> eq ==> eq ==> iff as wf_exp_eq_morph.
+#[export]
+Hint Resolve presup_ctx_sub : mcltt.
+
+Lemma presup_ctx_sub_left : forall {Γ Δ}, {{ ⊢ Γ ⊆ Δ }} -> {{ ⊢ Γ }}.
+Proof with easy.
+  intros * ?%presup_ctx_sub...
+Qed.
+
+#[export]
+Hint Resolve presup_ctx_sub_left : mcltt.
+
+Lemma presup_ctx_sub_right : forall {Γ Δ}, {{ ⊢ Γ ⊆ Δ }} -> {{ ⊢ Δ }}.
+Proof with easy.
+  intros * ?%presup_ctx_sub...
+Qed.
+
+#[export]
+Hint Resolve presup_ctx_sub_right : mcltt.
+
+Lemma presup_subtyp_right : forall {Γ A B}, {{ Γ ⊢ A ⊆ B }} -> exists i, {{ Γ ⊢ B : Type@i }}.
+Proof with mautosolve.
+  induction 1...
+Qed.
+
+#[export]
+Hint Resolve presup_subtyp_right : mcltt.
+
+(** Subtyping Rules without Extra Arguments *)
+
+Lemma wf_exp_subtyp' : forall Γ A A' M,
+    {{ Γ ⊢ M : A }} ->
+    {{ Γ ⊢ A ⊆ A' }} ->
+    {{ Γ ⊢ M : A' }}.
 Proof.
-  intros; split; mauto.
+  intros.
+  assert (exists i, {{ Γ ⊢ A' : Type@i }}) as [] by mauto.
+  econstructor; mauto.
+Qed.
+
+#[export]
+Hint Resolve wf_exp_subtyp' : mcltt.
+#[export]
+Remove Hints wf_exp_subtyp : mcltt.
+
+Lemma wf_sub_subtyp' : forall Γ Δ Δ' σ,
+    {{ Γ ⊢s σ : Δ }} ->
+    {{ ⊢ Δ ⊆ Δ' }} ->
+    {{ Γ ⊢s σ : Δ' }}.
+Proof.
+  intros.
+  econstructor; mauto.
+Qed.
+
+#[export]
+Hint Resolve wf_sub_subtyp' : mcltt.
+#[export]
+Remove Hints wf_sub_subtyp : mcltt.
+
+Lemma wf_exp_eq_subtyp' : forall Γ A A' M M',
+    {{ Γ ⊢ M ≈ M' : A }} ->
+    {{ Γ ⊢ A ⊆ A' }} ->
+    {{ Γ ⊢ M ≈ M' : A' }}.
+Proof.
+  intros.
+  assert (exists i, {{ Γ ⊢ A' : Type@i }}) as [] by mauto.
+  econstructor; mauto.
+Qed.
+
+#[export]
+Hint Resolve wf_exp_eq_subtyp' : mcltt.
+#[export]
+Remove Hints wf_exp_eq_subtyp : mcltt.
+
+Lemma wf_sub_eq_subtyp' : forall Γ Δ Δ' σ σ',
+    {{ Γ ⊢s σ ≈ σ' : Δ }} ->
+    {{ ⊢ Δ ⊆ Δ' }} ->
+    {{ Γ ⊢s σ ≈ σ' : Δ' }}.
+Proof.
+  intros.
+  econstructor; mauto.
+Qed.
+
+#[export]
+Hint Resolve wf_sub_eq_subtyp' : mcltt.
+#[export]
+Remove Hints wf_sub_eq_subtyp : mcltt.
+
+Add Parametric Morphism Γ T : (wf_exp_eq Γ T)
+    with signature wf_exp_eq Γ T ==> eq ==> iff as wf_exp_eq_morphism_iff1.
+Proof.
+  split; mauto.
 Qed.
 
 Add Parametric Morphism Γ T : (wf_exp_eq Γ T)
-    with signature (wf_exp_eq Γ T) ==> eq ==> iff as wf_exp_eq_morph1.
+    with signature eq ==> wf_exp_eq Γ T ==> iff as wf_exp_eq_morphism_iff2.
 Proof.
-  intros; split; mauto.
+  split; mauto.
 Qed.
 
-Add Parametric Morphism Γ T : (wf_exp_eq Γ T)
-    with signature eq ==> (wf_exp_eq Γ T) ==> iff as wf_exp_eq_morph2.
+Add Parametric Morphism Γ Δ : (wf_sub_eq Γ Δ)
+    with signature wf_sub_eq Γ Δ ==> eq ==> iff as wf_sub_eq_morphism_iff1.
 Proof.
-  intros; split; mauto.
+  split; mauto.
+Qed.
+
+Add Parametric Morphism Γ Δ : (wf_sub_eq Γ Δ)
+    with signature eq ==> wf_sub_eq Γ Δ ==> iff as wf_sub_eq_morphism_iff2.
+Proof.
+  split; mauto.
 Qed.
 
 #[export]
@@ -410,35 +541,18 @@ Hint Rewrite -> wf_sub_eq_id_compose_right wf_sub_eq_id_compose_left
                   wf_sub_eq_compose_assoc (* prefer right association *)
                   wf_sub_eq_p_extend using mauto 4 : mcltt.
 
+#[export]
+Hint Rewrite -> wf_exp_eq_sub_id wf_exp_eq_pi_sub using mauto 4 : mcltt.
 
 #[export]
- Hint Rewrite -> wf_exp_eq_sub_id wf_exp_eq_pi_sub using mauto 4 : mcltt.
-
-#[export]
-  Instance wf_exp_eq_per_elem Γ T : PERElem _ (wf_exp Γ T) (wf_exp_eq Γ T).
+Instance wf_exp_eq_per_elem Γ T : PERElem _ (wf_exp Γ T) (wf_exp_eq Γ T).
 Proof.
   intros a Ha. mauto.
 Qed.
 
 
 #[export]
-  Instance wf_sub_eq_per_elem Γ Δ : PERElem _ (wf_sub Γ Δ) (wf_sub_eq Γ Δ).
+Instance wf_sub_eq_per_elem Γ Δ : PERElem _ (wf_sub Γ Δ) (wf_sub_eq Γ Δ).
 Proof.
   intros a Ha. mauto.
-Qed.
-
-
-Add Parametric Morphism Γ j : (wf_subtyping Γ)
-    with signature eq ==> (wf_exp_eq Γ {{{Type@j}}}) ==> iff as wf_subtyping_resp_exp_eq_morphism1.
-Proof.
-  split; intros;
-    etransitivity; mauto 3.
-Qed.
-
-
-Add Parametric Morphism Γ i : (wf_subtyping Γ)
-    with signature (wf_exp_eq Γ {{{Type@i}}}) ==> eq ==> iff as wf_subtyping_resp_exp_eq_morphism2.
-Proof.
-  split; intros;
-    etransitivity; mauto 3.
 Qed.
