theories/Core/Completeness/LogicalRelation/Definitions.v
@@ -45,7 +45,7 @@ Hint Transparent valid_sub_under_ctx : mcltt.
 #[export]
 Hint Unfold valid_sub_under_ctx : mcltt.
 
-Definition sub_typ_under_ctx Γ M M' :=
+Definition subtyp_under_ctx Γ M M' :=
   exists env_rel (_ : {{ EF Γ ≈ Γ ∈ per_ctx_env ↘ env_rel }}) i,
   forall p p' (equiv_p_p' : {{ Dom p ≈ p' ∈ env_rel }}),
     exists R R', rel_typ i M p M p' R /\ rel_typ i M' p M' p' R' /\ rel_exp M p M' p' (per_subtyp i).
@@ -53,7 +53,7 @@ Definition sub_typ_under_ctx Γ M M' :=
 Notation "⊨ Γ ≈ Γ'" := (per_ctx Γ Γ')  (in custom judg at level 80, Γ custom exp, Γ' custom exp).
 Notation "⊨ Γ" := (valid_ctx Γ) (in custom judg at level 80, Γ custom exp).
 Notation "Γ ⊨ M ≈ M' : A" := (rel_exp_under_ctx Γ A M M') (in custom judg at level 80, Γ custom exp, M custom exp, M' custom exp, A custom exp).
-Notation "Γ ⊨ M ⊆ M'" := (sub_typ_under_ctx Γ M M') (in custom judg at level 80, Γ custom exp, M custom exp, M' custom exp).
+Notation "Γ ⊨ M ⊆ M'" := (subtyp_under_ctx Γ M M') (in custom judg at level 80, Γ custom exp, M custom exp, M' custom exp).
 Notation "Γ ⊨ M : A" := (valid_exp_under_ctx Γ A M) (in custom judg at level 80, Γ custom exp, M custom exp, A custom exp).
 Notation "Γ ⊨s σ ≈ σ' : Δ" := (rel_sub_under_ctx Γ Δ σ σ') (in custom judg at level 80, Γ custom exp, σ custom exp, σ' custom exp, Δ custom exp).
 Notation "Γ ⊨s σ : Δ" := (valid_sub_under_ctx Γ Δ σ) (in custom judg at level 80, Γ custom exp, σ custom exp, Δ custom exp).
